Suite et fin des structs comme r-values.  Ajout du type 'bool' et de l'operateur boolval.  Divers nettoyages
git-svn-id: https://yquem.inria.fr/compcert/svn/compcert/branches/volatiles@1805 fca1b0fc-160b-0410-b1d3-a4f43f01ea2e

backend/PrintCminor.ml
@@ -58,6 +58,7 @@ let name_of_unop = function
   | Ocast16unsigned -> "int16u"
   | Ocast16signed -> "int16s"
   | Onegint -> "-"
+  | Oboolval -> "(_Bool)"
   | Onotbool -> "!"
   | Onotint -> "~"
   | Onegf -> "-f"
